veric/semax_call.v
@@ -1346,7 +1346,7 @@ forall (Delta : tycontext) (A : TypeTree)
  (H0 : rho = construct_rho (filter_genv psi) vx tx)
  (H3 : eval_expr a rho = Vptr b Ptrofs.zero)
  (H4 : (funassert Delta rho) (m_phi jm))
- (H1 : (rguard Espec psi (fun _ => Delta)
+ (H1 : (rguard Espec psi Delta
         (frame_ret_assert R F0) k) (level (m_phi jm)))
  (H11 : forall vl : environ, (!|>(Q' ts x vl <=> Q ts x vl)) (m_phi jm))
  (H14 : (|>(F0 rho * F rho *
@@ -2159,7 +2159,7 @@ Lemma semax_call_aux:
     (*filter_genv psi = ge_of rho ->*)
     eval_expr a rho = Vptr b Ptrofs.zero ->
     (funassert Delta rho) (m_phi jm) ->
-    (rguard Espec psi (fun _ => Delta) (frame_ret_assert R F0) k) (level (m_phi jm)) ->
+    (rguard Espec psi Delta (frame_ret_assert R F0) k) (level (m_phi jm)) ->
     (believe Espec Delta psi Delta) (level (m_phi jm)) ->
     (glob_specs Delta)!id = Some (mk_funspec fsig0 cc A P Q' NEP NEQ') ->
     Genv.find_symbol psi id = Some b ->
